Refine.thy
@@ -2,55 +2,45 @@ theory Refine
   imports Language
 begin
 
-type_synonym tassn = "trace \<Rightarrow> bool"
-(*
-fun traceblock_extends :: "gstate rel \<Rightarrow> trace_block \<Rightarrow> trace_block \<Rightarrow> bool" where
-  "traceblock_extends \<alpha> (WaitBlock d1 p1 r1) (WaitBlock d2 p2 r2) =
-     (d1 \<le> d2 \<and> r1 = r2 \<and> (\<forall>t\<in>{0..d1}. (p1 t, p2 t) \<in> \<alpha>))"
-| "traceblock_extends _ b1 b2 = (b1 = b2)"
-
-definition strel_trans_single :: "state rel \<Rightarrow> gstate rel" where 
-  "strel_trans_single \<alpha> = {(State s1, State s2) | s1 s2. (s1, s2) \<in> \<alpha>}"
-
-definition traceblock_extends_single :: "state rel \<Rightarrow> trace_block \<Rightarrow> trace_block \<Rightarrow> bool" where  
-  "traceblock_extends_single \<alpha> t1 t2 = traceblock_extends (strel_trans_single \<alpha>) t1 t2"
-
-fun trace_extends :: "gstate rel \<Rightarrow> trace \<Rightarrow> trace \<Rightarrow> bool" where
-  "trace_extends \<alpha> [] [] = True"
-| "trace_extends \<alpha> (b1 # tr1) (b2 # tr2) = (
-     traceblock_extends \<alpha> b1 b2 \<and> trace_extends \<alpha> tr1 tr2
-   )"
-| "trace_extends _ _ _ = False"
-
-definition trace_extends_single :: "state rel \<Rightarrow> trace \<Rightarrow> trace \<Rightarrow> bool"
-  where "trace_extends_single \<alpha> = trace_extends (strel_trans_single \<alpha>)"
-
-lemma trace_extends_append: "\<lbrakk>trace_extends \<alpha> l1 l1'; trace_extends \<alpha> l2 l2'\<rbrakk> \<Longrightarrow> 
-      trace_extends \<alpha> (l1 @ l2) (l1' @ l2')"
-  sorry
-*)
-
-fun tblk_extends_single :: "state rel \<Rightarrow> trace_block \<Rightarrow> trace_block \<Rightarrow> bool" where
-  "tblk_extends_single \<alpha> (WaitBlock d1 p1 r1) (WaitBlock d2 p2 r2) = (
-     d1 \<le> d2 \<and> r1 = r2 \<and> (\<forall>t\<in>{0..d1}.
+fun tblk_single :: "state rel \<Rightarrow> trace_block \<Rightarrow> trace_block \<Rightarrow> bool" where
+  "tblk_single \<alpha> (WaitBlock d1 p1 r1) (WaitBlock d2 p2 r2) = (
+     d1 = d2 \<and> r1 = r2 \<and> (\<forall>t\<in>{0..d1}.
        (\<exists>s1 s2. p1 t = State s1 \<and> p2 t = State s2 \<and> (s1, s2) \<in> \<alpha>)
      ))"
-| "tblk_extends_single _ b1 b2 = (b1 = b2)"
+| "tblk_single _ b1 b2 = (b1 = b2)"
 
-lemma tblk_extends_single_weaken:
+lemma restrict_iff: "(\<lambda>\<tau>\<in>{0..d}. p \<tau>) = (\<lambda>\<tau>\<in>{0..d}. p' \<tau>) \<longleftrightarrow> (\<forall>t. 0 \<le> t \<and> t \<le> d \<longrightarrow> p t = p' t)"
+  by (metis atLeastAtMost_iff restrict_apply' restrict_ext)
+
+lemma tblk_single_Id:
+  assumes "wf_tblk_single blk1" "wf_tblk_single blk2"
+      and "tblk_single Id blk1 blk2"
+    shows "blk1 = blk2"
+proof(cases blk1)
+  case (CommBlock x11 x12 x13)
+  with assms(3) show ?thesis by simp
+next
+  case (WaitBlock d p1 r)
+  with assms(3) obtain p2 where "blk2 = WaitBlock d p2 r \<and> (\<forall>t\<in>{0..d}. p1 t = p2 t)"
+    by (smt (verit) pair_in_Id_conv tblk_single.elims(2) trace_block.inject(2))
+  with assms(1,2) show ?thesis
+    using WaitBlock wf_tblk_single.simps(1) by force
+qed
+
+lemma tblk_single_weaken:
   assumes "\<alpha> \<subseteq> \<beta>"
-      and "tblk_extends_single \<alpha> blk1 blk2"
-    shows "tblk_extends_single \<beta> blk1 blk2"
+      and "tblk_single \<alpha> blk1 blk2"
+    shows "tblk_single \<beta> blk1 blk2"
   using assms
   apply (cases blk1, cases blk2, simp_all)
   apply (cases blk2, simp)
   apply auto
   by (meson atLeastAtMost_iff subsetD)
 
-lemma tblk_extends_single_refl:
+lemma tblk_single_refl:
   assumes "refl \<alpha>"
       and "wf_tblk_single blk"
-  shows "tblk_extends_single \<alpha> blk blk"
+  shows "tblk_single \<alpha> blk blk"
 proof(cases blk)
   case (CommBlock c ch v)
   then show ?thesis by auto
@@ -60,64 +50,119 @@ next
     using assms(1) assms(2) reflD by fastforce
 qed
 
-lemma tblk_extends_single_compose:
-  assumes "tblk_extends_single \<alpha> blk1 blk2"
-      and "tblk_extends_single \<beta> blk2 blk3"
-    shows "tblk_extends_single (\<alpha> O \<beta>) blk1 blk3"
+lemma tblk_single_compose:
+  assumes "tblk_single \<alpha> blk1 blk2"
+      and "tblk_single \<beta> blk2 blk3"
+    shows "tblk_single (\<alpha> O \<beta>) blk1 blk3"
   using assms
   apply (cases blk1, cases blk2, cases blk3, simp_all)
   apply (cases blk2, cases blk3, simp_all)
   apply (cases blk3, simp)
   apply auto
   by (metis (no_types, opaque_lifting) atLeastAtMost_iff gstate.inject(1) 
-      order.trans relcomp.relcompI)
+      relcomp.relcompI)
 
-lemma tblk_extends_single_trans:
+lemma tblk_single_trans:
   assumes "trans \<alpha>"
-      and "tblk_extends_single \<alpha> blk1 blk2"
-      and "tblk_extends_single \<alpha> blk2 blk3"
-    shows "tblk_extends_single \<alpha> blk1 blk3"
+      and "tblk_single \<alpha> blk1 blk2"
+      and "tblk_single \<alpha> blk2 blk3"
+    shows "tblk_single \<alpha> blk1 blk3"
   using assms
-  by (meson tblk_extends_single_compose tblk_extends_single_weaken trans_O_subset)
+  by (meson tblk_single_compose tblk_single_weaken trans_O_subset)
 
-definition tr_extends_single :: "state rel \<Rightarrow> trace \<Rightarrow> trace \<Rightarrow> bool" where
-  "tr_extends_single \<alpha> tr1 tr2 \<equiv> list_all2 (tblk_extends_single \<alpha>) tr1 tr2"
+definition tr_single :: "state rel \<Rightarrow> trace \<Rightarrow> trace \<Rightarrow> bool" where
+  "tr_single \<alpha> tr1 tr2 \<equiv> list_all2 (tblk_single \<alpha>) tr1 tr2"
 
-lemma tr_extends_single_weaken:
+lemma tr_single_Id:
+  assumes "tr_single Id tr1 tr2"
+      and "wf_tr_single tr1" "wf_tr_single tr2"
+    shows "tr1 = tr2"
+  using assms
+proof(induct tr1 arbitrary: tr2)
+  case Nil
+  then show ?case
+    by (simp add: tr_single_def)
+next
+  case (Cons blk1 tr1)
+  then obtain blk2 tr2' where a0: "tr2 = blk2 # tr2'" "tr_single Id tr1 tr2'" "tblk_single Id blk1 blk2"
+    by (metis list_all2_Cons1 tr_single_def)
+  with Cons.hyps Cons.prems(2,3) have a1: "tr1 = tr2'"
+    using  wf_tr_single_def by auto
+  from a0(1,3) Cons.prems(2,3) have "blk1 = blk2"
+    using tblk_single_Id wf_tr_single_def by auto
+  with a1 a0(1) show ?case by simp
+qed
+
+lemma tr_single_weaken:
   assumes "\<alpha> \<subseteq> \<beta>"
-      and "tr_extends_single \<alpha> tr1 tr2"
-    shows "tr_extends_single \<beta> tr1 tr2"
+      and "tr_single \<alpha> tr1 tr2"
+    shows "tr_single \<beta> tr1 tr2"
   using assms
-  by (metis list_all2_conv_all_nth tblk_extends_single_weaken tr_extends_single_def)
+  by (metis list_all2_conv_all_nth tblk_single_weaken tr_single_def)
 
-lemma tr_extends_single_refl:
+lemma tr_single_refl:
   assumes "refl \<alpha>"
       and "wf_tr_single tr"
-    shows "tr_extends_single \<alpha> tr tr"
+    shows "tr_single \<alpha> tr tr"
   using assms
-  by (simp add: list_all2_conv_all_nth list_all_length tblk_extends_single_refl 
-      tr_extends_single_def)
+  by (metis in_set_conv_decomp list.rel_refl_strong list_all_append list_all_simps(1) 
+      tblk_single_refl tr_single_def wf_tr_single_def)
 
-lemma tr_extends_single_compose:
+lemma tr_single_compose:
   assumes "trans \<alpha>"
-      and "tr_extends_single \<alpha> tr1 tr2"
-      and "tr_extends_single \<beta> tr2 tr3"
-    shows "tr_extends_single (\<alpha> O \<beta>) tr1 tr3"
+      and "tr_single \<alpha> tr1 tr2"
+      and "tr_single \<beta> tr2 tr3"
+    shows "tr_single (\<alpha> O \<beta>) tr1 tr3"
   using assms
-  by (smt (verit, best) list_all2_conv_all_nth tblk_extends_single_compose tr_extends_single_def)
+  by (smt (verit, best) list_all2_conv_all_nth tblk_single_compose tr_single_def)
 
-lemma tr_extends_single_trans:
+lemma tr_single_trans:
   assumes "trans \<alpha>"
-      and "tr_extends_single \<alpha> tr1 tr2"
-      and "tr_extends_single \<alpha> tr2 tr3"
-    shows "tr_extends_single \<alpha> tr1 tr3"
+      and "tr_single \<alpha> tr1 tr2"
+      and "tr_single \<alpha> tr2 tr3"
+    shows "tr_single \<alpha> tr1 tr3"
   using assms
-  by (meson tr_extends_single_compose tr_extends_single_weaken trans_O_subset)
+  by (meson tr_single_compose tr_single_weaken trans_O_subset)
   
 definition hybrid_sim_single :: "proc \<Rightarrow> state \<Rightarrow> (state rel) \<Rightarrow> proc \<Rightarrow> state \<Rightarrow> bool" 
   ("'(_, _') \<sqsubseteq> _ '(_, _')") where
-  "(P\<^sub>c, s\<^sub>c) \<sqsubseteq> \<alpha> (P\<^sub>a, s\<^sub>a) = (\<forall>s\<^sub>c' tr\<^sub>c. big_step P\<^sub>c s\<^sub>c tr\<^sub>c s\<^sub>c' \<longrightarrow> (s\<^sub>c, s\<^sub>a) \<in> \<alpha> \<and>
-   (\<exists>s\<^sub>a' tr\<^sub>a. big_step P\<^sub>a s\<^sub>a tr\<^sub>a s\<^sub>a' \<and> tr_extends_single \<alpha> tr\<^sub>c tr\<^sub>a \<and> (s\<^sub>c', s\<^sub>a') \<in> \<alpha>))"
+  "(P\<^sub>c, s\<^sub>c) \<sqsubseteq> \<alpha> (P\<^sub>a, s\<^sub>a) = ((s\<^sub>c, s\<^sub>a) \<in> \<alpha> \<and> (\<forall>s\<^sub>c' tr\<^sub>c. big_step P\<^sub>c s\<^sub>c tr\<^sub>c s\<^sub>c' \<longrightarrow> 
+   (\<exists>s\<^sub>a' tr\<^sub>a. big_step P\<^sub>a s\<^sub>a tr\<^sub>a s\<^sub>a' \<and> tr_single \<alpha> tr\<^sub>c tr\<^sub>a \<and> (s\<^sub>c', s\<^sub>a') \<in> \<alpha>)))"
+
+definition hybrid_equiv_single :: "proc \<Rightarrow> state \<Rightarrow> (state rel) \<Rightarrow> proc \<Rightarrow> state \<Rightarrow> bool"
+  ("'(_, _') \<sim> _ '(_, _')") where
+  "(P\<^sub>c, s\<^sub>c) \<sim> \<alpha> (P\<^sub>a, s\<^sub>a) = ((P\<^sub>c, s\<^sub>c) \<sqsubseteq> \<alpha> (P\<^sub>a, s\<^sub>a) \<and> (P\<^sub>a, s\<^sub>a) \<sqsubseteq> \<alpha> (P\<^sub>c, s\<^sub>c))"
+ 
+theorem hybrid_sim_single_Id:
+  "(P\<^sub>c, s\<^sub>c) \<sqsubseteq> Id (P\<^sub>a, s\<^sub>a) \<longleftrightarrow> (s\<^sub>c = s\<^sub>a \<and> (\<forall>s\<^sub>c' tr\<^sub>c. big_step P\<^sub>c s\<^sub>c tr\<^sub>c s\<^sub>c' \<longrightarrow> big_step P\<^sub>a s\<^sub>a tr\<^sub>c s\<^sub>c'))"
+  by (metis (no_types, lifting) hybrid_sim_single_def pair_in_Id_conv proc_wf_tr_single refl_Id tr_single_Id tr_single_refl)
+
+theorem hybrid_equiv_single_Id:
+  "(P\<^sub>c, s\<^sub>c) \<sim> Id (P\<^sub>a, s\<^sub>a)  \<longleftrightarrow> (s\<^sub>c = s\<^sub>a \<and> (\<forall>s\<^sub>c' tr\<^sub>c. big_step P\<^sub>c s\<^sub>c tr\<^sub>c s\<^sub>c' \<longleftrightarrow> big_step P\<^sub>a s\<^sub>a tr\<^sub>c s\<^sub>c'))"
+  by (meson hybrid_equiv_single_def hybrid_sim_single_Id)  
+
+theorem equiv_Id_single_refl:
+  assumes "(P\<^sub>c, s\<^sub>c) \<sim> Id (P\<^sub>a, s\<^sub>a)"
+  shows "(P\<^sub>a, s\<^sub>a) \<sim> Id (P\<^sub>c, s\<^sub>c)"
+  using assms hybrid_equiv_single_Id by auto
+
+lemma big_step_skipl: "big_step P s tr s' \<longleftrightarrow> big_step (Skip; P) s tr s'"
+  by (metis append_self_conv2 seqB seqE skipB skipE)
+
+lemma big_step_skipr: "big_step P s tr s' \<longleftrightarrow> big_step (P; Skip) s tr s'"
+  by (metis append_Nil2 seqB seqE skipB skipE)
+
+theorem equiv_Id_single_skipl: "(P, s) \<sim> Id (Skip; P, s)"
+  using big_step_skipl hybrid_equiv_single_Id by force
+
+theorem equiv_Id_single_skipr: "(P, s) \<sim> Id (P; Skip, s)"
+  using big_step_skipr hybrid_equiv_single_Id by presburger
+
+lemma big_step_seq_assoc: "big_step ((C1; C2); C3) s tr s' \<longleftrightarrow> big_step (C1; (C2; C3)) s tr s'"
+  by (smt (verit, ccfv_SIG) append.assoc seqB seqE)
+
+theorem equiv_Id_single_seq: "((C1; C2); C3, s) \<sim> Id (C1; (C2; C3), s)"
+  by (simp add: big_step_seq_assoc hybrid_equiv_single_Id)
 
 definition reachable :: "proc \<Rightarrow> state \<Rightarrow> state \<Rightarrow> bool" where
   "reachable C s s' = (\<exists>tr. big_step C s tr s')"
@@ -130,20 +175,20 @@ theorem sim_weaken:
       and "(P\<^sub>c, s\<^sub>c) \<sqsubseteq> \<alpha> (P\<^sub>a, s\<^sub>a)"
     shows "(P\<^sub>c, s\<^sub>c) \<sqsubseteq> \<beta> (P\<^sub>a, s\<^sub>a)"
   using assms hybrid_sim_single_def
-  by (meson subsetD tr_extends_single_weaken)
+  by (meson subsetD tr_single_weaken)
 
 theorem sim_refl: 
   assumes "refl \<alpha>"
   shows "(C, s) \<sqsubseteq> \<alpha> (C, s)"
   using assms hybrid_sim_single_def
-  by (meson proc_wf_tr_single reflD tr_extends_single_refl)
+  by (meson proc_wf_tr_single reflD tr_single_refl)
 
 theorem sim_compose:
   assumes "(P\<^sub>c, s\<^sub>c) \<sqsubseteq> \<alpha> (P\<^sub>m, s\<^sub>m)"
       and "(P\<^sub>m, s\<^sub>m) \<sqsubseteq> \<beta> (P\<^sub>a, s\<^sub>a)"
     shows "(P\<^sub>c, s\<^sub>c) \<sqsubseteq> (\<alpha> O \<beta>) (P\<^sub>a, s\<^sub>a)"
   using assms hybrid_sim_single_def
-  by (smt (verit) list_all2_trans relcomp.simps tblk_extends_single_compose tr_extends_single_def)
+  by (smt (verit) list_all2_trans relcomp.simps tblk_single_compose tr_single_def)
 
 theorem sim_trans:
   assumes "trans \<alpha>"
@@ -160,7 +205,7 @@ theorem sim_havoc:
   using assms
   apply (simp add: hybrid_sim_single_def, clarify)
   apply (rule_tac x = "s\<^sub>a (y := v)" in exI)
-  apply (rule_tac x = tr\<^sub>c in exI, simp add: tr_extends_single_def)
+  apply (rule_tac x = tr\<^sub>c in exI, simp add: tr_single_def)
   using HavocB assignE by blast
 
 corollary sim_havoc_Id: "((x ::= e), s) \<sqsubseteq> Id ((x ::= *), s)"
@@ -184,7 +229,7 @@ theorem sim_ichoice_r:
   assumes "(P\<^sub>c, s\<^sub>c) \<sqsubseteq> \<alpha> (P\<^sub>a\<^sub>1, s\<^sub>a) \<or> (P\<^sub>c, s\<^sub>c) \<sqsubseteq> \<alpha> (P\<^sub>a\<^sub>2, s\<^sub>a)"
   shows "(P\<^sub>c, s\<^sub>c) \<sqsubseteq> \<alpha> (IChoice P\<^sub>a\<^sub>1 P\<^sub>a\<^sub>2, s\<^sub>a)"
   using assms
-  apply (simp add: hybrid_sim_single_def, clarify)
+  apply (simp add: hybrid_sim_single_def)
   using IChoiceB1 IChoiceB2 by blast
 
 corollary sim_ichoice_r_Id:
@@ -198,7 +243,7 @@ theorem sim_assume:
   shows "(Assume b\<^sub>c, s\<^sub>c) \<sqsubseteq> \<alpha> (Assume b\<^sub>a, s\<^sub>a)"
   using assms
   apply (simp add: hybrid_sim_single_def, clarify)
-  by (metis AssumeB AssumeE list_all2_Nil2 tr_extends_single_def)
+  by (metis AssumeB AssumeE list_all2_Nil2 tr_single_def)
   
 corollary sim_assume_Id:
   assumes "b1 s \<longrightarrow> b2 s"
@@ -217,16 +262,16 @@ proof-
       then obtain s\<^sub>c\<^sub>m tr\<^sub>c\<^sub>1 tr\<^sub>c\<^sub>2 where a0: "big_step P\<^sub>c\<^sub>1 s\<^sub>c tr\<^sub>c\<^sub>1 s\<^sub>c\<^sub>m" "big_step P\<^sub>c\<^sub>2 s\<^sub>c\<^sub>m tr\<^sub>c\<^sub>2 s\<^sub>c'" "tr\<^sub>c = tr\<^sub>c\<^sub>1 @ tr\<^sub>c\<^sub>2"
         by (meson seqE)
       from a0(1) assms(2) obtain s\<^sub>a\<^sub>m tr\<^sub>a\<^sub>1 where a1: "big_step P\<^sub>a\<^sub>1 s\<^sub>a tr\<^sub>a\<^sub>1 s\<^sub>a\<^sub>m" 
-      "tr_extends_single \<alpha> tr\<^sub>c\<^sub>1 tr\<^sub>a\<^sub>1" "(s\<^sub>c\<^sub>m, s\<^sub>a\<^sub>m) \<in> \<alpha>"
-        using hybrid_sim_single_def by blast       
+      "tr_single \<alpha> tr\<^sub>c\<^sub>1 tr\<^sub>a\<^sub>1" "(s\<^sub>c\<^sub>m, s\<^sub>a\<^sub>m) \<in> \<alpha>"
+        by (metis hybrid_sim_single_def)      
       from assms(3) a0(1) a0(2) a1(3) obtain s\<^sub>a' tr\<^sub>a\<^sub>2 where "big_step P\<^sub>a\<^sub>2 s\<^sub>a\<^sub>m tr\<^sub>a\<^sub>2 s\<^sub>a'"
-      "tr_extends_single \<alpha> tr\<^sub>c\<^sub>2 tr\<^sub>a\<^sub>2" "(s\<^sub>c', s\<^sub>a') \<in> \<alpha>"
+      "tr_single \<alpha> tr\<^sub>c\<^sub>2 tr\<^sub>a\<^sub>2" "(s\<^sub>c', s\<^sub>a') \<in> \<alpha>"
         by (metis hybrid_sim_single_def reachable_def)
-      with a0(3) a1(1) a1(2) have "\<exists>tr\<^sub>a s\<^sub>a'. big_step (P\<^sub>a\<^sub>1; P\<^sub>a\<^sub>2) s\<^sub>a tr\<^sub>a s\<^sub>a' \<and> tr_extends_single \<alpha> tr\<^sub>c tr\<^sub>a \<and> (s\<^sub>c', s\<^sub>a') \<in> \<alpha>"
-        by (metis list_all2_appendI seqB tr_extends_single_def)
+      with a0(3) a1(1) a1(2) have "\<exists>tr\<^sub>a s\<^sub>a'. big_step (P\<^sub>a\<^sub>1; P\<^sub>a\<^sub>2) s\<^sub>a tr\<^sub>a s\<^sub>a' \<and> tr_single \<alpha> tr\<^sub>c tr\<^sub>a \<and> (s\<^sub>c', s\<^sub>a') \<in> \<alpha>"
+        by (metis list_all2_appendI seqB tr_single_def)
     }
     with assms(1) show ?thesis
-      using hybrid_sim_single_def by blast      
+      by (metis hybrid_sim_single_def)          
   qed
 
 corollary sim_seq_Id:
@@ -235,46 +280,74 @@ corollary sim_seq_Id:
     shows "(P\<^sub>c\<^sub>1;P\<^sub>c\<^sub>2, s) \<sqsubseteq> Id (P\<^sub>a\<^sub>1; P\<^sub>a\<^sub>2, s)"
   by (rule sim_seq, simp_all add: assms)
 
-(*
-theorem sim_loop_l:
-  assumes "(s\<^sub>c, s\<^sub>a) \<in> \<alpha>" "trans \<alpha>"
-      and "\<forall>s\<^sub>c' s\<^sub>a'. reachable (Rep P\<^sub>c\<^sub>1) s\<^sub>c s\<^sub>c' \<longrightarrow> (s\<^sub>c', s\<^sub>a') \<in> \<alpha> \<longrightarrow> (P\<^sub>c\<^sub>1; P\<^sub>a, s\<^sub>c') \<sqsubseteq> \<alpha> (P\<^sub>a, s\<^sub>a')"
-      and "\<forall>s\<^sub>c' s\<^sub>a'. reachable (Rep P\<^sub>c\<^sub>1) s\<^sub>c s\<^sub>c' \<longrightarrow> (s\<^sub>c', s\<^sub>a') \<in> \<alpha> \<longrightarrow> (P\<^sub>c\<^sub>2, s\<^sub>c') \<sqsubseteq> \<alpha> (P\<^sub>a, s\<^sub>a')"
-    shows "(Rep P\<^sub>c\<^sub>1; P\<^sub>c\<^sub>2, s\<^sub>c) \<sqsubseteq> \<alpha> (P\<^sub>a, s\<^sub>a)"
-proof-
-  from assms have "(P\<^sub>c\<^sub>1; P\<^sub>a, s\<^sub>c) \<sqsubseteq> \<alpha> (P\<^sub>a, s\<^sub>a)"
-    using RepetitionB1 reachable_def by blast
+theorem sim_loop_l_Id:
+  assumes "\<forall>s'. reachable (Rep P\<^sub>c\<^sub>1) s s' \<longrightarrow> (P\<^sub>c\<^sub>1; P\<^sub>a, s') \<sqsubseteq> Id (P\<^sub>a, s')"
+      and "\<forall>s'. reachable (Rep P\<^sub>c\<^sub>1) s s' \<longrightarrow> (P\<^sub>c\<^sub>2, s') \<sqsubseteq> Id (P\<^sub>a, s')"
+    shows "(Rep P\<^sub>c\<^sub>1; P\<^sub>c\<^sub>2, s) \<sqsubseteq> Id (P\<^sub>a, s)"
 proof-
   {
-    fix s\<^sub>c' tr\<^sub>c
-    assume "big_step (Rep P\<^sub>c\<^sub>1; P\<^sub>c\<^sub>2) s\<^sub>c tr\<^sub>c s\<^sub>c'"
-    then obtain s\<^sub>c\<^sub>m tr\<^sub>c\<^sub>1 tr\<^sub>c\<^sub>2 where a0: "big_step (Rep P\<^sub>c\<^sub>1) s\<^sub>c tr\<^sub>c\<^sub>1 s\<^sub>c\<^sub>m" "big_step P\<^sub>c\<^sub>2 s\<^sub>c\<^sub>m tr\<^sub>c\<^sub>2 s\<^sub>c'" "tr\<^sub>c = tr\<^sub>c\<^sub>1 @ tr\<^sub>c\<^sub>2"
+    fix s' tr
+    assume "big_step (Rep P\<^sub>c\<^sub>1; P\<^sub>c\<^sub>2) s tr s'"
+    then obtain sm tr1 tr2 where a0: "big_step (Rep P\<^sub>c\<^sub>1) s tr1 sm" "big_step P\<^sub>c\<^sub>2 sm tr2 s'" "tr = tr1 @ tr2"
       by (meson seqE)
-    then obtain n where a1: "iterate_bigstep n (s\<^sub>c, []) P\<^sub>c\<^sub>1 (s\<^sub>c\<^sub>m, tr\<^sub>c\<^sub>1)"
+    with assms(2) have a1: "big_step P\<^sub>a sm tr2 s'"
+      using hybrid_sim_single_Id reachable_def by auto
+    from a0(1) obtain n where "iterate_bigstep n (s, []) P\<^sub>c\<^sub>1 (sm, tr1)"
       by (metis append_Nil big_step_while)
-    with a0(2) a0(3) have "\<exists>s\<^sub>a' tr\<^sub>a. big_step P\<^sub>a s\<^sub>a tr\<^sub>a s\<^sub>a' \<and> tr_extends_single \<alpha> tr\<^sub>c tr\<^sub>a \<and> (s\<^sub>c', s\<^sub>a') \<in> \<alpha>"
+    with a0(3) a1 have "big_step P\<^sub>a s tr s'"
+    proof(induct n arbitrary: sm tr1 tr2)
       case 0
-      then have b0: "s\<^sub>c = s\<^sub>c\<^sub>m \<and> tr\<^sub>c\<^sub>1 = []"
+      with assms(2) show ?case
         by simp
-      from assms(4) assms(1) have "(P\<^sub>c\<^sub>2, s\<^sub>c) \<sqsubseteq> \<alpha> (P\<^sub>a, s\<^sub>a)"
-        using RepetitionB1 reachable_def sorry
-      with b0 obtain s\<^sub>a' tr\<^sub>a where "big_step P\<^sub>a s\<^sub>a tr\<^sub>a s\<^sub>a' \<and> tr_extends_single \<alpha> tr\<^sub>c tr\<^sub>a \<and> (s\<^sub>c', s\<^sub>a') \<in> \<alpha>"
-        by (metis "0.prems"(1) a0(3) hybrid_sim_single_def self_append_conv2)
-      then show ?case
-        by auto        
     next
       case (Suc n)
-      from Suc.prems(3) obtain s\<^sub>c\<^sub>m\<^sub>1 tr\<^sub>c\<^sub>m\<^sub>1 tr\<^sub>c\<^sub>m\<^sub>2 where c0: "big_step P\<^sub>c\<^sub>1 s\<^sub>c tr\<^sub>c\<^sub>m\<^sub>1 s\<^sub>c\<^sub>m\<^sub>1"
-      "iterate_bigstep n (s\<^sub>c\<^sub>m\<^sub>1, []) P\<^sub>c\<^sub>1 (s\<^sub>c\<^sub>m, tr\<^sub>c\<^sub>m\<^sub>2)" "tr\<^sub>c\<^sub>1 = tr\<^sub>c\<^sub>m\<^sub>1 @ tr\<^sub>c\<^sub>m\<^sub>2"
-        by (metis append_Nil iterate_bigstep_converse iterate_bigstep_init')       
-      with Suc.prems(1) Suc.hyps           
-      then show ?case sorry
+      from Suc.prems(3) obtain sm1 trm1 trm2 where b0: "iterate_bigstep n (s, []) P\<^sub>c\<^sub>1 (sm1, trm1)"
+      "big_step P\<^sub>c\<^sub>1 sm1 trm2 sm" "tr1 = trm1 @ trm2"
+        by auto
+      with Suc.prems(2) have "big_step (P\<^sub>c\<^sub>1; P\<^sub>a) sm1 (trm2 @ tr2) s'"
+        using seqB by auto
+      with b0(1) assms(1) have "big_step P\<^sub>a sm1 (trm2 @ tr2) s'"
+        by (metis append_Nil big_step_while hybrid_sim_single_Id reachable_def)
+      with b0(1,3) Suc.prems(1) Suc.hyps[of trm1 "trm2 @ tr2" sm1] show ?case by auto
     qed
   }
-  with assms(1) show ?thesis
-    by (simp add: hybrid_sim_single_def)
+  then show ?thesis
+    using hybrid_sim_single_Id by force
 qed
-*)
+
+theorem sim_loop_r_Id:
+  assumes "(P\<^sub>c\<^sub>2, s) \<sqsubseteq> Id (P\<^sub>a, s)"
+      and "(P\<^sub>a; P\<^sub>c\<^sub>1, s) \<sqsubseteq> Id (P\<^sub>a, s)"
+    shows "(P\<^sub>c\<^sub>2; Rep P\<^sub>c\<^sub>1, s) \<sqsubseteq> Id (P\<^sub>a, s)"
+proof-
+  {
+    fix s' tr
+    assume "big_step (P\<^sub>c\<^sub>2; Rep P\<^sub>c\<^sub>1) s tr s'"
+    then obtain sm tr1 tr2 where a0: "big_step P\<^sub>c\<^sub>2 s tr1 sm" "big_step (Rep P\<^sub>c\<^sub>1) sm tr2 s'" "tr = tr1 @ tr2"
+      by (meson seqE)
+    with assms(1) have a1: "big_step P\<^sub>a s tr1 sm"
+      by (simp add: hybrid_sim_single_Id)
+    from a0(2,3) obtain n where "iterate_bigstep n (sm, tr1) P\<^sub>c\<^sub>1 (s', tr)"
+      by (metis big_step_while)
+    with  a1 have "big_step P\<^sub>a s tr s'"
+    proof(induct n arbitrary: sm tr1 tr2)
+      case 0
+      then show ?case by simp
+    next
+      case (Suc n)
+      from Suc.prems(2) obtain sm1 trm1 where b0: "big_step P\<^sub>c\<^sub>1 sm trm1 sm1" 
+      "iterate_bigstep n (sm1, tr1 @ trm1) P\<^sub>c\<^sub>1 (s', tr)"
+        using iterate_bigstep_converse by blast
+      with Suc.prems(1) have "big_step (P\<^sub>a; P\<^sub>c\<^sub>1) s (tr1 @ trm1) sm1"
+        by (simp add: seqB)
+      with assms(2) have "big_step P\<^sub>a s (tr1 @ trm1) sm1"
+        by (simp add: hybrid_sim_single_Id)
+      with b0(2) Suc.hyps[of "tr1 @ trm1" sm1] show ?case by auto
+    qed
+  }
+  then show ?thesis
+    using hybrid_sim_single_Id by force
+qed
 
 theorem sim_unloop:
   assumes "(s\<^sub>c, s\<^sub>a) \<in> \<alpha>"
@@ -286,31 +359,31 @@ proof-
     assume "big_step (Rep P\<^sub>c) s\<^sub>c tr\<^sub>c s\<^sub>c'"
     then obtain n where "iterate_bigstep n (s\<^sub>c, []) P\<^sub>c (s\<^sub>c', tr\<^sub>c)"
       by (metis append_Nil big_step_while)
-    then have "\<exists>s\<^sub>a' tr\<^sub>a. big_step (Rep P\<^sub>a) s\<^sub>a tr\<^sub>a s\<^sub>a' \<and> tr_extends_single \<alpha> tr\<^sub>c tr\<^sub>a \<and> (s\<^sub>c', s\<^sub>a') \<in> \<alpha>"
+    then have "\<exists>s\<^sub>a' tr\<^sub>a. big_step (Rep P\<^sub>a) s\<^sub>a tr\<^sub>a s\<^sub>a' \<and> tr_single \<alpha> tr\<^sub>c tr\<^sub>a \<and> (s\<^sub>c', s\<^sub>a') \<in> \<alpha>"
     proof(induct n arbitrary: s\<^sub>c' tr\<^sub>c)
       case 0
       then have "s\<^sub>c = s\<^sub>c' \<and> tr\<^sub>c = []"
         by simp
       with assms(1) show ?case
-        by (rule_tac x = s\<^sub>a in exI, rule_tac x = "[]" in exI, simp add: RepetitionB1 tr_extends_single_def) 
+        by (rule_tac x = s\<^sub>a in exI, rule_tac x = "[]" in exI, simp add: RepetitionB1 tr_single_def) 
     next
       case (Suc n)
       from Suc.prems obtain s\<^sub>c\<^sub>m tr\<^sub>c\<^sub>1 tr\<^sub>c\<^sub>2 where b0: "iterate_bigstep n (s\<^sub>c, []) P\<^sub>c (s\<^sub>c\<^sub>m, tr\<^sub>c\<^sub>1)"
       "big_step P\<^sub>c s\<^sub>c\<^sub>m tr\<^sub>c\<^sub>2 s\<^sub>c'" "tr\<^sub>c = tr\<^sub>c\<^sub>1 @ tr\<^sub>c\<^sub>2"
         by auto
       with Suc.hyps[of s\<^sub>c\<^sub>m tr\<^sub>c\<^sub>1] obtain s\<^sub>a\<^sub>m tr\<^sub>a\<^sub>1 where b1: "big_step (Rep P\<^sub>a) s\<^sub>a tr\<^sub>a\<^sub>1 s\<^sub>a\<^sub>m" 
-           "tr_extends_single \<alpha> tr\<^sub>c\<^sub>1 tr\<^sub>a\<^sub>1" "(s\<^sub>c\<^sub>m, s\<^sub>a\<^sub>m) \<in> \<alpha>"
+           "tr_single \<alpha> tr\<^sub>c\<^sub>1 tr\<^sub>a\<^sub>1" "(s\<^sub>c\<^sub>m, s\<^sub>a\<^sub>m) \<in> \<alpha>"
         by auto
       from b0(1) b0(2) assms(2) b1(3) obtain tr\<^sub>a\<^sub>2 s\<^sub>a' where b2: "big_step P\<^sub>a s\<^sub>a\<^sub>m tr\<^sub>a\<^sub>2 s\<^sub>a'" 
-           "tr_extends_single \<alpha> tr\<^sub>c\<^sub>2 tr\<^sub>a\<^sub>2" "(s\<^sub>c', s\<^sub>a') \<in> \<alpha>"
+           "tr_single \<alpha> tr\<^sub>c\<^sub>2 tr\<^sub>a\<^sub>2" "(s\<^sub>c', s\<^sub>a') \<in> \<alpha>"
         by (metis big_step_while hybrid_sim_single_def reachable_def self_append_conv2)
       with b0(3) b1 show ?case
         by (rule_tac x = s\<^sub>a' in exI, rule_tac x = "tr\<^sub>a\<^sub>1 @ tr\<^sub>a\<^sub>2" in exI, simp add: 
-               big_step_RepetitionB3 tr_extends_single_def list_all2_appendI)
+               big_step_RepetitionB3 tr_single_def list_all2_appendI)
     qed
   }
   with assms(1) show ?thesis
-    using hybrid_sim_single_def by blast
+    using hybrid_sim_single_def by force
 qed
 
 theorem sim_unloop_Id:
@@ -319,6 +392,8 @@ theorem sim_unloop_Id:
   by (rule sim_unloop, simp_all add: assms)
 
 text \<open>ODE with invariant\<close>
+type_synonym tassn = "trace \<Rightarrow> bool"
+
 inductive ode_inv_assn :: "(state \<Rightarrow> bool) \<Rightarrow> tassn" where
   "\<forall>t\<in>{0..d::real}. f (p t) \<Longrightarrow> ode_inv_assn f [WaitBlk d (\<lambda>\<tau>. State (p \<tau>)) ({}, {})]"
 
@@ -352,9 +427,301 @@ proof-
     qed
   }
   then show ?thesis
-    by (meson hybrid_sim_single_def pair_in_Id_conv proc_wf_tr_single refl_Id tr_extends_single_refl)
+    by (meson hybrid_sim_single_def pair_in_Id_conv proc_wf_tr_single refl_Id tr_single_refl)
 qed
 
+fun tblk_par :: "gstate rel \<Rightarrow> trace_block \<Rightarrow> trace_block \<Rightarrow> bool" where
+  "tblk_par \<alpha> (WaitBlock d1 p1 r1) (WaitBlock d2 p2 r2) =
+     (d1 = d2 \<and> r1 = r2 \<and> (\<forall>t\<in>{0..d1}. (p1 t, p2 t) \<in> \<alpha>))"
+| "tblk_par _ b1 b2 = (b1 = b2)"
+
+lemma tblk_par_waitblk:
+  assumes "tblk_par \<alpha> (WaitBlock d p r) blk"
+      and "wf_tblk_par blk"
+    shows "\<exists>p'. blk = WaitBlk d p' r \<and> (\<forall>t\<in>{0..d}. (p t, p' t) \<in> \<alpha>)"
+proof-
+  from assms(1) obtain p' where "blk = WaitBlock d p' r" "\<forall>t\<in>{0..d}. (p t, p' t) \<in> \<alpha>"
+    using tblk_par.elims(2) by force
+  with assms(2) show ?thesis
+    using WaitBlk_def by auto
+qed
+
+lemma tblk_par_waitblk':
+  assumes "tblk_par \<alpha> (WaitBlk d p r) blk"
+      and "wf_tblk_par blk"
+    shows "\<exists>p'. blk = WaitBlk d p' r \<and> (\<forall>t\<in>{0..d}. (p t, p' t) \<in> \<alpha>)"
+  by (smt (verit) WaitBlk_def assms(1,2) restrict_def tblk_par_waitblk)
+
+lemma tblk_par_weaken:
+  assumes "\<alpha> \<subseteq> \<beta>"
+      and "tblk_par \<alpha> blk1 blk2"
+    shows "tblk_par \<beta> blk1 blk2"
+  using assms
+  apply (cases blk1, cases blk2, simp_all)
+  apply (cases blk2, simp)
+  by auto
+
+lemma tblk_par_refl:
+  assumes "refl \<alpha>"
+  shows "tblk_par \<alpha> blk blk"
+proof(cases blk)
+  case (CommBlock c ch v)
+  then show ?thesis by auto
+next
+  case (WaitBlock d p r)
+  then show ?thesis
+    using assms(1) reflD by fastforce
+qed
+
+lemma tblk_par_compose:
+  assumes "tblk_par \<alpha> blk1 blk2"
+      and "tblk_par \<beta> blk2 blk3"
+    shows "tblk_par (\<alpha> O \<beta>) blk1 blk3"
+  using assms
+  apply (cases blk1, cases blk2, cases blk3, simp_all)
+  apply (cases blk2, cases blk3, simp_all)
+  apply (cases blk3, simp)
+  by auto
+
+lemma tblk_par_trans:
+  assumes "trans \<alpha>"
+      and "tblk_par \<alpha> blk1 blk2"
+      and "tblk_par \<alpha> blk2 blk3"
+    shows "tblk_par \<alpha> blk1 blk3"
+  using assms
+  by (meson tblk_par_compose tblk_par_weaken trans_O_subset)
+
+definition tr_par :: "gstate rel \<Rightarrow> trace \<Rightarrow> trace \<Rightarrow> bool" where
+  "tr_par \<alpha> tr1 tr2 = list_all2 (tblk_par \<alpha>) tr1 tr2"
+
+lemma tr_par_weaken:
+  assumes "\<alpha> \<subseteq> \<beta>"
+      and "tr_par \<alpha> tr1 tr2"
+    shows "tr_par \<beta> tr1 tr2"
+  using assms
+  by (simp add: list_all2_conv_all_nth tblk_par_weaken tr_par_def)
+
+lemma tr_par_refl:
+  assumes "refl \<alpha>"
+    shows "tr_par \<alpha> tr tr"
+  using assms
+  by (simp add: list_all2_conv_all_nth tblk_par_refl tr_par_def)
+
+lemma tr_par_compose:
+  assumes "trans \<alpha>"
+      and "tr_par \<alpha> tr1 tr2"
+      and "tr_par \<beta> tr2 tr3"
+    shows "tr_par (\<alpha> O \<beta>) tr1 tr3"
+  using assms
+  by (smt (verit, best) list_all2_trans tblk_par_compose tr_par_def)
+
+lemma tr_par_trans:
+  assumes "trans \<alpha>"
+      and "tr_par \<alpha> tr1 tr2"
+      and "tr_par \<alpha> tr2 tr3"
+    shows "tr_par \<alpha> tr1 tr3"
+  using assms
+  using tr_par_compose tr_par_weaken trans_O_subset by blast
+  
+definition hybrid_sim_par :: "pproc \<Rightarrow> gstate \<Rightarrow> (gstate rel) \<Rightarrow> pproc \<Rightarrow> gstate \<Rightarrow> bool" 
+  ("'(_, _') \<sqsubseteq>\<^sub>p _ '(_, _')") where
+  "(P\<^sub>c, s\<^sub>c) \<sqsubseteq>\<^sub>p \<alpha> (P\<^sub>a, s\<^sub>a) = (\<forall>s\<^sub>c' tr\<^sub>c. par_big_step P\<^sub>c s\<^sub>c tr\<^sub>c s\<^sub>c' \<longrightarrow> (s\<^sub>c, s\<^sub>a) \<in> \<alpha> \<and>
+   (\<exists>s\<^sub>a' tr\<^sub>a. par_big_step P\<^sub>a s\<^sub>a tr\<^sub>a s\<^sub>a' \<and> tr_par \<alpha> tr\<^sub>c tr\<^sub>a \<and> (s\<^sub>c', s\<^sub>a') \<in> \<alpha>))"
+
+definition lift_rel_single :: "(state rel) \<Rightarrow> (gstate rel)" ( "\<Up>\<^sub>s _" [80] 80) where 
+  "\<Up>\<^sub>s \<alpha> = {(State s1, State s2) |s1 s2. (s1, s2) \<in> \<alpha>}"
+
+definition lift_rel_par :: "(gstate rel) \<Rightarrow> (gstate rel) \<Rightarrow> (gstate rel)" (infixr "\<uplus>\<^sub>p" 80) where 
+  "\<alpha> \<uplus>\<^sub>p \<beta> = {(ParState s1 s2, ParState s1' s2') |s1 s2 s1' s2'. (s1, s1') \<in> \<alpha> \<and> (s2, s2') \<in> \<beta>}"
+
+lemma tblk_lift_rel_single:
+  assumes "tblk_single \<alpha> tr1 tr2"
+    shows "tblk_par (\<Up>\<^sub>s \<alpha>) tr1 tr2"
+  using assms
+  apply (cases tr1, cases tr2, simp_all)
+  by (cases tr2, simp_all add: lift_rel_single_def)
+
+lemma tr_lift_rel_single:
+  assumes "tr_single \<alpha> tr1 tr2"
+  shows "tr_par (\<Up>\<^sub>s \<alpha>) tr1 tr2"
+  by (metis assms list_all2_mono tblk_lift_rel_single tr_par_def tr_single_def)
+
+lemma tr_par_cons_waitblk:
+  assumes "tr_par \<alpha> ((WaitBlk d p rdy) # blks) tr'"
+      and "wf_tr_par tr'"
+    shows "\<exists>p' blks'. tr' = (WaitBlk d p' rdy) # blks' \<and> (\<forall>t\<in>{0..d}. (p t, p' t) \<in> \<alpha>) \<and> tr_par \<alpha> blks blks'"
+proof-
+  from assms(1) obtain wait blks' where a0: "tr' = wait # blks'" "tr_par \<alpha> blks blks'"
+  "tblk_par \<alpha> (WaitBlk d p rdy) wait"
+    by (metis list_all2_Cons1 tr_par_def)
+  with assms(2) have "wf_tblk_par wait"
+    using wf_tr_par_cons by blast
+  with a0(3) obtain p' where "wait = WaitBlk d p' rdy" "\<forall>t\<in>{0..d}. (p t, p' t) \<in> \<alpha>"
+    by (metis tblk_par_waitblk')
+  with a0 show ?thesis
+    by auto
+qed
+
+lemma restrict_slide:
+  assumes "t1 < t2" "t1 > 0"
+      and "(\<lambda>\<tau>\<in>{0..t2}. p \<tau>) = (\<lambda>\<tau>\<in>{0..t2}. p' \<tau>)"
+    shows "(\<lambda>\<tau>\<in>{0..t2 - t1}. p (\<tau> + t1)) = (\<lambda>\<tau>\<in>{0..t2 - t1}. p (\<tau> + t1))"
+  by blast
+
+lemma wf_tblk_par_slide:
+  assumes "wf_tblk_par (WaitBlk t2 p rdy)"
+      and "t1 > 0"
+    shows "wf_tblk_par (WaitBlk (t2 - t1) (\<lambda> \<tau>. p(\<tau> + t1)) rdy)"
+  using assms
+  apply (simp add: WaitBlk_def, clarsimp)
+  apply (rule_tac x = "\<lambda>\<tau>. f (\<tau> + t1)" in exI)
+  by (simp add: restrict_iff)
+
+lemma tr_combine_sim: 
+  assumes "combine_blocks chs tr1 tr2 tr3"
+      and "tr_par \<alpha> tr1 tr1'"
+      and "tr_par \<beta> tr2 tr2'"
+      and "wf_tr_par tr1'"
+      and "wf_tr_par tr2'"
+    shows "\<exists>tr3'. combine_blocks chs tr1' tr2' tr3' \<and> tr_par (\<alpha> \<uplus>\<^sub>p \<beta>) tr3 tr3'"
+  using assms
+proof(induction arbitrary: tr1' tr2' rule: combine_blocks.induct)
+  case (combine_blocks_empty comms)
+  then show ?case 
+    by (simp add: combine_blocks.combine_blocks_empty tr_par_def)
+next
+  case (combine_blocks_pair1 ch comms blks1 blks2 blks v)
+  then obtain blks1' blks2' where a0: "tr1' = InBlock ch v # blks1'" "tr_par \<alpha> blks1 blks1'"
+  "tr2' = OutBlock ch v # blks2'" "tr_par \<beta> blks2 blks2'"
+    by (metis list_all2_Cons1 tblk_par.simps(2) tr_par_def)
+  with combine_blocks_pair1.IH obtain blks' where "combine_blocks comms blks1' blks2' blks'" 
+  "tr_par (\<alpha> \<uplus>\<^sub>p \<beta>) blks blks'"
+    using combine_blocks_pair1.prems(3,4) wf_tr_par_cons by blast
+  with combine_blocks_pair1.hyps(1) a0 show ?case
+    using combine_blocks.combine_blocks_pair1[of ch comms blks1' blks2' blks' v] tr_par_def by auto
+next
+  case (combine_blocks_pair2 ch comms blks1 blks2 blks v)
+  then obtain blks1' blks2' where b0: "tr1' = OutBlock ch v # blks1'" "tr_par \<alpha> blks1 blks1'"
+  "tr2' = InBlock ch v # blks2'" "tr_par \<beta> blks2 blks2'"
+    by (metis list_all2_Cons1 tblk_par.simps(2) tr_par_def)
+  with combine_blocks_pair2.IH obtain blks' where "combine_blocks comms blks1' blks2' blks'" 
+  "tr_par (\<alpha> \<uplus>\<^sub>p \<beta>) blks blks'"
+    using combine_blocks_pair2.prems(3,4) wf_tr_par_cons by blast
+  with combine_blocks_pair2.hyps(1) b0 show ?case
+    using combine_blocks.combine_blocks_pair2[of ch comms blks1' blks2' blks' v] tr_par_def by auto
+next
+  case (combine_blocks_unpair1 ch comms blks1 blks2 blks ch_type v)
+  then obtain blks1' where c0: "tr1' = CommBlock ch_type ch v # blks1'" "tr_par \<alpha> blks1 blks1'"
+    by (metis list_all2_Cons1 tblk_par.simps(2) tr_par_def)
+  with combine_blocks_unpair1.IH[of blks1' tr2'] obtain blks' where 
+  "combine_blocks comms blks1' tr2' blks'" "tr_par (\<alpha> \<uplus>\<^sub>p \<beta>) blks blks'"
+    using combine_blocks_unpair1.prems(2,3,4) wf_tr_par_cons by blast
+  with c0 combine_blocks_unpair1.hyps(1) show ?case
+    using combine_blocks.combine_blocks_unpair1[of ch comms blks1' tr2' blks' ch_type v] tr_par_def by auto
+next
+  case (combine_blocks_unpair2 ch comms blks1 blks2 blks ch_type v)
+  then obtain blks2' where d0: "tr2' = CommBlock ch_type ch v # blks2'" "tr_par \<beta> blks2 blks2'"
+    by (metis list_all2_Cons1 tblk_par.simps(2) tr_par_def)
+  with combine_blocks_unpair2.IH[of tr1' blks2'] obtain blks' where
+  "combine_blocks comms tr1' blks2' blks'" "tr_par (\<alpha> \<uplus>\<^sub>p \<beta>) blks blks'"
+    using combine_blocks_unpair2.prems(1,3,4) wf_tr_par_cons by blast
+  with d0 combine_blocks_unpair2.hyps(1) show ?case
+    using combine_blocks.combine_blocks_unpair2[of ch comms tr1' blks2' blks' ch_type v] tr_par_def by auto
+next
+  case (combine_blocks_wait1 comms blks1 blks2 blks rdy1 rdy2 hist hist1 hist2 rdy d)
+  then obtain hist1' blks1' hist2' blks2' where e0:
+  "tr1' = (WaitBlk d hist1' rdy1) # blks1'" "tr_par \<alpha> blks1 blks1'" "\<forall>t\<in>{0..d}. (hist1 t, hist1' t) \<in> \<alpha>"
+  "tr2' = (WaitBlk d hist2' rdy2) # blks2'" "tr_par \<beta> blks2 blks2'" "\<forall>t\<in>{0..d}. (hist2 t, hist2' t) \<in> \<beta>"
+    by (metis (lifting) tr_par_cons_waitblk)
+  with combine_blocks_wait1.IH obtain blks' where e1: "combine_blocks comms blks1' blks2' blks'"
+    "tr_par (\<alpha> \<uplus>\<^sub>p \<beta>) blks blks'"
+    using combine_blocks_wait1.prems(3,4) wf_tr_par_cons by blast
+  from e0(3,6) combine_blocks_wait1.hyps(3) have 
+    "tblk_par (\<alpha> \<uplus>\<^sub>p \<beta>) (WaitBlk d hist rdy) (WaitBlk d (\<lambda>\<tau>. ParState (hist1' \<tau>) (hist2' \<tau>)) rdy)"
+    by (simp add: WaitBlk_def lift_rel_par_def restrict_def)
+  with e0 e1 combine_blocks_wait1.hyps show ?case
+    using combine_blocks.combine_blocks_wait1[of comms blks1' blks2' blks' rdy1 rdy2
+    "\<lambda>\<tau>. ParState (hist1' \<tau>) (hist2' \<tau>)" hist1' hist2' rdy d]
+    using tr_par_def by auto
+next
+  case (combine_blocks_wait2 comms blks1 t2 t1 hist2 rdy2 blks2 blks rdy1 hist hist1 rdy)
+  then obtain hist1' blks1' hist2' blks2' where f0:
+  "tr1' = (WaitBlk t1 hist1' rdy1) # blks1'" "tr_par \<alpha> blks1 blks1'" "\<forall>t\<in>{0..t1}. (hist1 t, hist1' t) \<in> \<alpha>"
+  "tr2' = (WaitBlk t2 hist2' rdy2) # blks2'"  "tr_par \<beta> blks2 blks2'" "\<forall>t\<in>{0..t2}. (hist2 t, hist2' t) \<in> \<beta>"
+    by (metis (no_types, opaque_lifting) tr_par_cons_waitblk)
+  then have f1: "tr_par \<beta> (WaitBlk (t2 - t1) (\<lambda>\<tau>. hist2 (\<tau> + t1)) rdy2 # blks2) (WaitBlk (t2 - t1) (\<lambda>\<tau>. hist2' (\<tau> + t1)) rdy2 # blks2')"
+    by (simp add: WaitBlk_def tr_par_def combine_blocks_wait2.hyps(4) order_less_imp_le)
+  with combine_blocks_wait2.IH combine_blocks_wait2.prems(3,4) f0 obtain blks' where f2:
+  "combine_blocks comms blks1' (WaitBlk (t2 - t1) (\<lambda>\<tau>. hist2' (\<tau> + t1)) rdy2 # blks2') blks'"
+  "tr_par (\<alpha> \<uplus>\<^sub>p \<beta>) blks blks'"
+    by (metis WaitBlk_def list_all_simps(1) wf_tblk_par.simps(1) wf_tr_par_def)
+  from f0(3,6) \<open>t1 < t2\<close>  have "tblk_par (\<alpha> \<uplus>\<^sub>p \<beta>) (WaitBlk t1 hist rdy) (WaitBlk t1 (\<lambda>\<tau>. ParState (hist1' \<tau>) (hist2' \<tau>)) rdy)"
+    by (simp add: WaitBlk_def combine_blocks_wait2.hyps(5) lift_rel_par_def)
+  with f0 f1 f2 combine_blocks_wait2.hyps show ?case 
+    using combine_blocks.combine_blocks_wait2[of comms blks1' t2 t1 hist2' rdy2 blks2' blks' rdy1 
+    "\<lambda>\<tau>. ParState (hist1' \<tau>) (hist2' \<tau>)" hist1' rdy] tr_par_def by auto
+next
+  case (combine_blocks_wait3 comms t1 t2 hist1 rdy1 blks1 blks2 blks rdy2 hist hist2 rdy)
+  then obtain hist1' blks1' hist2' blks2' where g0:
+  "tr1' = (WaitBlk t1 hist1' rdy1) # blks1'" "tr_par \<alpha> blks1 blks1'" "\<forall>t\<in>{0..t1}. (hist1 t, hist1' t) \<in> \<alpha>" 
+  "tr2' = (WaitBlk t2 hist2' rdy2) # blks2'" "tr_par \<beta> blks2 blks2'" "\<forall>t\<in>{0..t2}. (hist2 t, hist2' t) \<in> \<beta>"
+    by (metis (no_types, opaque_lifting) tr_par_cons_waitblk)
+  then have g1: "tr_par \<alpha> (WaitBlk (t1 - t2) (\<lambda>\<tau>. hist1 (\<tau> + t2)) rdy1 # blks1) (WaitBlk (t1 - t2) (\<lambda>\<tau>. hist1' (\<tau> + t2)) rdy1 # blks1')"
+    by (simp add: WaitBlk_def tr_par_def combine_blocks_wait3.hyps(4) order_less_imp_le)
+  with combine_blocks_wait3.IH g0(1,4,5) combine_blocks_wait3.prems(3,4) obtain blks' where g2:
+    "combine_blocks comms (WaitBlk (t1 - t2) (\<lambda>\<tau>. hist1' (\<tau> + t2)) rdy1 # blks1') blks2' blks'"
+    "tr_par (\<alpha> \<uplus>\<^sub>p \<beta>) blks blks'"
+    by (metis WaitBlk_def list_all_simps(1) wf_tblk_par.simps(1) wf_tr_par_def)
+  from g0(3,6) \<open>t2 < t1\<close>  have "tblk_par (\<alpha> \<uplus>\<^sub>p \<beta>) (WaitBlk t2 hist rdy) (WaitBlk t2 (\<lambda>\<tau>. ParState (hist1' \<tau>) (hist2' \<tau>)) rdy)"
+    by (simp add: WaitBlk_def combine_blocks_wait3.hyps(5) lift_rel_par_def)
+  with g0 g1 g2 combine_blocks_wait3.hyps show ?case 
+    using combine_blocks.combine_blocks_wait3[of comms t1 t2 hist1' rdy1 blks1' blks2' blks' rdy2
+    "\<lambda>\<tau>. ParState (hist1' \<tau>) (hist2' \<tau>)" hist2' rdy]
+    tr_par_def by auto
+qed
+
+theorem sim_Single:
+  assumes "(P\<^sub>c, s\<^sub>c) \<sqsubseteq> \<alpha> (P\<^sub>a, s\<^sub>a)"
+  shows "(Single P\<^sub>c, State s\<^sub>c) \<sqsubseteq>\<^sub>p \<Up>\<^sub>s \<alpha> (Single P\<^sub>a, State s\<^sub>a)"
+proof-
+  {
+    fix s' tr\<^sub>c
+    assume "par_big_step (Single P\<^sub>c) (State s\<^sub>c) tr\<^sub>c s'"
+    then obtain s\<^sub>c' where a0: "big_step P\<^sub>c s\<^sub>c tr\<^sub>c s\<^sub>c'" "s' = State s\<^sub>c'"
+      by (metis SingleE gstate.inject(1))
+    with assms obtain s\<^sub>a' tr\<^sub>a where "big_step P\<^sub>a s\<^sub>a tr\<^sub>a s\<^sub>a'" "(s\<^sub>c, s\<^sub>a) \<in> \<alpha>" "(s\<^sub>c', s\<^sub>a') \<in> \<alpha>"
+    "tr_single \<alpha> tr\<^sub>c tr\<^sub>a"
+      by (meson hybrid_sim_single_def)
+    with a0 have "(State s\<^sub>c, State s\<^sub>a) \<in> \<Up>\<^sub>s \<alpha> \<and> (\<exists>s'' tr\<^sub>a. par_big_step (Single P\<^sub>a) (State s\<^sub>a) tr\<^sub>a s'' 
+     \<and> tr_par (\<Up>\<^sub>s \<alpha>) tr\<^sub>c tr\<^sub>a \<and> (s', s'') \<in> \<Up>\<^sub>s \<alpha>)"
+      by (metis (mono_tags, lifting) CollectI SingleB lift_rel_single_def tr_lift_rel_single)
+  }
+  then show ?thesis
+    by (simp add: hybrid_sim_par_def)
+qed
+
+theorem sim_Par:
+  assumes "(P\<^sub>c\<^sub>1, s\<^sub>c\<^sub>1) \<sqsubseteq>\<^sub>p \<alpha> (P\<^sub>a\<^sub>1, s\<^sub>a\<^sub>1)"
+      and "(P\<^sub>c\<^sub>2, s\<^sub>c\<^sub>2) \<sqsubseteq>\<^sub>p \<beta> (P\<^sub>a\<^sub>2, s\<^sub>a\<^sub>2)"
+    shows "(Parallel P\<^sub>c\<^sub>1 chs P\<^sub>c\<^sub>2, ParState s\<^sub>c\<^sub>1 s\<^sub>c\<^sub>2) \<sqsubseteq>\<^sub>p \<alpha> \<uplus>\<^sub>p \<beta> (Parallel P\<^sub>a\<^sub>1 chs P\<^sub>a\<^sub>2, ParState s\<^sub>a\<^sub>1 s\<^sub>a\<^sub>2)"
+proof-
+  {
+    fix s\<^sub>c' tr\<^sub>c
+    assume "par_big_step (Parallel P\<^sub>c\<^sub>1 chs P\<^sub>c\<^sub>2) (ParState s\<^sub>c\<^sub>1 s\<^sub>c\<^sub>2) tr\<^sub>c s\<^sub>c'"
+    then obtain s\<^sub>c\<^sub>1' s\<^sub>c\<^sub>2' tr\<^sub>c\<^sub>1 tr\<^sub>c\<^sub>2 where a0: "par_big_step P\<^sub>c\<^sub>1 s\<^sub>c\<^sub>1 tr\<^sub>c\<^sub>1 s\<^sub>c\<^sub>1'" "par_big_step P\<^sub>c\<^sub>2 s\<^sub>c\<^sub>2 tr\<^sub>c\<^sub>2 s\<^sub>c\<^sub>2'"
+    "combine_blocks chs tr\<^sub>c\<^sub>1 tr\<^sub>c\<^sub>2 tr\<^sub>c" "s\<^sub>c' = ParState s\<^sub>c\<^sub>1' s\<^sub>c\<^sub>2'"
+      by (smt (verit, best) ParallelE gstate.inject(2))
+    with assms obtain s\<^sub>a\<^sub>1' s\<^sub>a\<^sub>2' tr\<^sub>a\<^sub>1 tr\<^sub>a\<^sub>2 where 
+    "(s\<^sub>c\<^sub>1, s\<^sub>a\<^sub>1) \<in> \<alpha> \<and> par_big_step P\<^sub>a\<^sub>1 s\<^sub>a\<^sub>1 tr\<^sub>a\<^sub>1 s\<^sub>a\<^sub>1' \<and> tr_par \<alpha> tr\<^sub>c\<^sub>1 tr\<^sub>a\<^sub>1 \<and> (s\<^sub>c\<^sub>1', s\<^sub>a\<^sub>1') \<in> \<alpha>"
+    "(s\<^sub>c\<^sub>2, s\<^sub>a\<^sub>2) \<in> \<beta> \<and> par_big_step P\<^sub>a\<^sub>2 s\<^sub>a\<^sub>2 tr\<^sub>a\<^sub>2 s\<^sub>a\<^sub>2' \<and> tr_par \<beta> tr\<^sub>c\<^sub>2 tr\<^sub>a\<^sub>2 \<and> (s\<^sub>c\<^sub>2', s\<^sub>a\<^sub>2') \<in> \<beta>"
+      by (meson hybrid_sim_par_def)
+    with a0 have "(ParState s\<^sub>c\<^sub>1 s\<^sub>c\<^sub>2, ParState s\<^sub>a\<^sub>1 s\<^sub>a\<^sub>2) \<in> \<alpha> \<uplus>\<^sub>p \<beta> \<and> 
+    (\<exists>s\<^sub>a' tr\<^sub>a. par_big_step (Parallel P\<^sub>a\<^sub>1 chs P\<^sub>a\<^sub>2) (ParState s\<^sub>a\<^sub>1 s\<^sub>a\<^sub>2) tr\<^sub>a s\<^sub>a' \<and> 
+     tr_par (\<alpha> \<uplus>\<^sub>p \<beta>) tr\<^sub>c tr\<^sub>a \<and> (s\<^sub>c', s\<^sub>a') \<in> \<alpha> \<uplus>\<^sub>p \<beta>)"
+      by (smt (verit, ccfv_threshold) ParallelB lift_rel_par_def mem_Collect_eq pproc_wf_tr_single tr_combine_sim)
+  }
+  then show ?thesis
+    using hybrid_sim_par_def by presburger
+qed
 
 end
-
